ArkLib/CommitmentScheme/InductiveMerkleTree.lean
@@ -10,6 +10,7 @@ import ArkLib.CommitmentScheme.Basic
 import Mathlib.Data.Vector.Snoc
 import ArkLib.CommitmentScheme.QueryCacheToSet
 import ArkLib.CommitmentScheme.BinaryTree
+import ArkLib.ToVCVio.Oracle
 
 /-!
 # Inductive Merkle Trees
@@ -113,6 +114,23 @@ def buildMerkleTree {s} (leaf_tree : LeafDataTree α s) : OracleComp (spec α) (
     let rootHash ← singleHash α leftTree.getRootValue rightTree.getRootValue
     return FullDataTree.internal rootHash leftTree rightTree
 
+lemma runWithOracle_buildMerkleTree {s} (leaf_data_tree : LeafDataTree α s) (f) :
+    (runWithOracle f (buildMerkleTree leaf_data_tree))
+    = buildMerkleTree_with_hash leaf_data_tree fun (left right : α) =>
+      (f () ⟨left, right⟩) := by
+  induction s with
+  | leaf =>
+    match leaf_data_tree with
+    | LeafDataTree.leaf a =>
+      unfold buildMerkleTree
+      simp only [runWithOracle_pure, buildMerkleTree_with_hash]
+  | internal s_left s_right left_ih right_ih =>
+    match leaf_data_tree with
+    | LeafDataTree.internal left right =>
+      unfold buildMerkleTree
+      simp [left_ih, right_ih, runWithOracle_bind]
+      rfl
+
 /-- Generate a Merkle proof for a leaf at a given idx
     The proof consists of the sibling hashes needed to recompute the root.
 -/
@@ -130,6 +148,13 @@ def generateProof {s} (cache_tree : FullDataTree α s) :
 theorem generateProof_ofLeaf {α : Type} (cache_tree : FullDataTree α Skeleton.leaf) :
     generateProof cache_tree SkeletonLeafIndex.ofLeaf = [] := by
   rfl
+
+@[simp]
+theorem generateProof_leaf {α : Type} (a : α) (idx) :
+    generateProof (FullDataTree.leaf a) idx = [] := by
+  cases idx with
+  | ofLeaf => rfl
+
 
 @[simp]
 theorem generateProof_ofLeft {α : Type} {sleft sright : Skeleton}
@@ -176,15 +201,61 @@ def getPutativeRoot {s} (idx : BinaryTree.SkeletonLeafIndex s) (leafValue : α)
       let ancestorBelowRootHash ← getPutativeRoot idxRight leafValue restProof
       singleHash α siblingBelowRootHash ancestorBelowRootHash
 
+def getPutativeRoot_with_hash {s} (idx : BinaryTree.SkeletonLeafIndex s)
+    (leafValue : α) (proof : List α) (hashFn : α → α → α) : α :=
+  match proof with
+  | [] => leafValue -- If no proof, the root is just the leaf value
+  | siblingBelowRootHash :: restProof =>
+    match idx with
+    | BinaryTree.SkeletonLeafIndex.ofLeaf =>
+      -- This indicates that the proof is longer than the depth of the tree, which is invalid.
+      -- A more well-typed version using `Vector` might prevent this.
+      -- For now, we just return the leaf value.
+      leafValue
+    | BinaryTree.SkeletonLeafIndex.ofLeft idxLeft =>
+      -- Recursively get the hash of the ancestor of the leaf which is just below the root
+      hashFn (getPutativeRoot_with_hash idxLeft leafValue restProof hashFn) siblingBelowRootHash
+    | BinaryTree.SkeletonLeafIndex.ofRight idxRight =>
+      -- Recursively get the hash of the ancestor of the leaf which is just below the root
+      hashFn siblingBelowRootHash (getPutativeRoot_with_hash idxRight leafValue restProof hashFn)
+
+lemma runWithOracle_getPutativeRoot {s} (idx : BinaryTree.SkeletonLeafIndex s)
+    (leafValue : α) (proof : List α) (f) :
+    (runWithOracle f (getPutativeRoot idx leafValue proof))
+    = getPutativeRoot_with_hash idx leafValue proof fun (left right : α) =>
+      (f () ⟨left, right⟩) := by
+  induction proof generalizing s with
+  | nil =>
+    unfold getPutativeRoot
+    simp only [runWithOracle_pure, getPutativeRoot_with_hash]
+  | cons siblingBelowRootHash restProof ih =>
+    unfold getPutativeRoot
+    cases s with
+    | leaf =>
+      cases idx with
+      | ofLeaf =>
+        rfl
+    | internal s_left s_right =>
+      cases idx with
+      | ofLeft idxLeft =>
+        simp [runWithOracle_bind, ih]
+        rfl
+      | ofRight idxRight =>
+        simp only [runWithOracle_bind, ih]
+        rfl
+
+end
+
 /-- Verify a Merkle proof `proof` that a given `leaf` at index `i` is in the Merkle tree with given
   `root`.
   Works by computing the putative root based on the branch, and comparing that to the actual root.
   Outputs `failure` if the proof is invalid. -/
-def verifyProof [DecidableEq α] {s}
+def verifyProof {α} [DecidableEq α] {s}
     (idx : BinaryTree.SkeletonLeafIndex s) (leafValue : α) (rootValue : α)
     (proof : List α) : OracleComp (spec α) Unit := do
   let putative_root ← getPutativeRoot idx leafValue proof
   guard (putative_root = rootValue)
+
 
 theorem singleHash_neverFails [DecidableEq α] [inst_1 : SelectableType α] (left right : α)
     (preexisting_cache : (spec α).QueryCache) :
@@ -199,59 +270,7 @@ theorem singleHash_neverFails [DecidableEq α] [inst_1 : SelectableType α] (lef
   | some u =>
     simp only [StateT.run_pure, neverFails_pure]
 
-theorem buildMerkleTree_neverFails {α : Type} [DecidableEq α] [SelectableType α] {s : Skeleton}
-    (leaf_tree : LeafDataTree α s) (preexisting_cache : (spec α).QueryCache) :
-    ((simulateQ randomOracle (buildMerkleTree leaf_tree)).run preexisting_cache).neverFails := by
-  induction leaf_tree generalizing preexisting_cache with
-  | leaf a =>
-    unfold buildMerkleTree
-    simp only [simulateQ_pure, StateT.run_pure, neverFails_pure]
-  | internal left right left_ih right_ih =>
-    unfold buildMerkleTree
-    simp [simulateQ_bind, StateT.run_bind, neverFails_bind_iff, left_ih, right_ih]
-    intro merkle_cache_left query_cache h_mem_support merkle_cache_right query_cache' h_mem_support'
-    clear left_ih right_ih
-    exact
-      singleHash_neverFails merkle_cache_left.getRootValue merkle_cache_right.getRootValue
-        query_cache'
 
-theorem getPutativeRoot_neverFails {α : Type} [inst : DecidableEq α] [inst_1 : SelectableType α]
-    {s : Skeleton} (idx : SkeletonLeafIndex s) (leafValue : α) (query_cache : (spec α).QueryCache)
-    (proof : List α) :
-    ((simulateQ randomOracle
-            (getPutativeRoot idx leafValue proof)).run
-        query_cache).neverFails := by
-  induction proof generalizing s idx leafValue query_cache with
-  | nil =>
-    unfold getPutativeRoot
-    simp only [simulateQ_pure, StateT.run_pure, neverFails_pure]
-  | cons siblingBelowRootHash restProof ih =>
-    unfold getPutativeRoot
-    cases s with
-    | leaf =>
-      cases idx with
-      | ofLeaf =>
-        -- If the index is a leaf, then the proof is invalid, so we just return the leaf value.
-        simp only [simulateQ_pure, StateT.run_pure, neverFails_pure]
-    | internal left right =>
-      cases idx with
-      | ofLeft idxLeft =>
-        simp only [simulateQ_bind, StateT.run_bind, neverFails_bind_iff]
-        constructor
-        · apply ih
-        · intro x x_mem
-          simp only [Function.comp_apply]
-          exact singleHash_neverFails x.1 siblingBelowRootHash x.2
-      | ofRight idxRight =>
-        simp only [simulateQ_bind, StateT.run_bind, neverFails_bind_iff]
-        constructor
-        · apply ih
-        · intro x x_mem
-          simp only [Function.comp_apply]
-          exact singleHash_neverFails siblingBelowRootHash x.1 x.2
-
-
--- To VCVio
 
 
 -- To Mathlib (the symmetric form of preexisting lemma)
@@ -354,441 +373,42 @@ theorem mem_singleHash_support_iff {α : Type} [DecidableEq α] [SelectableType 
       simp [h_eq]
 
 
-/-- Characterize membership in buildMerkleTree support
-
-A merkle_tree_cache, resulting_cache pair is in the support of the
-  buildMerkleTree on leaf_data_tree simulation starting from preexisting_cache
-  iff:
-
-1. Any entry is only in the resulting_cache iff it is either in the preexisting_cache
-   or in the merkle_tree_cache
-2. The leaves of the data tree are the same as the leaves of the merkle_tree_cache
-   (i.e. the merkle tree cache is a valid Merkle tree for the leaf data tree)
-3. The merkle_tree_cache is self consistent (i.e. any two nodes with children with the same values
-   have the value)
--/
-theorem mem_buildMerkleTree_support_iff_v2 {α : Type} [DecidableEq α] [SelectableType α]
-    {s : Skeleton}
-    (leaf_data_tree : LeafDataTree α s)
-    (merkle_tree_cache : FullDataTree α s)
-    (preexisting_cache resulting_cache : (spec α).QueryCache) :
-    ((merkle_tree_cache, resulting_cache)
-      ∈ ((simulateQ randomOracle (buildMerkleTree leaf_data_tree)).run preexisting_cache).support)
-    ↔
-    (
-      ∀ d r,
-        resulting_cache () d = some r ↔ (preexisting_cache () d = some r ∨ (d, r) ∈
-          merkle_tree_cache.toQueryCacheSet)
-    )
-    ∧
-    leaf_data_tree = merkle_tree_cache.toLeafDataTree
-    ∧
-    (
-      merkle_tree_cache.isSelfConsistent
-    )
-
-     := by
-  induction s generalizing preexisting_cache resulting_cache with
-  | leaf =>
-    cases leaf_data_tree with
-    | leaf a =>
-      unfold buildMerkleTree
-      simp only [simulateQ_pure, StateT.run_pure, support_pure, Set.mem_singleton_iff,
-        Prod.mk.injEq, domain_def, range_def, FullDataTree.leaf_toQueryCacheSet',
-        Set.mem_empty_iff_false, or_false, Option.eq_of_forall_eq, Prod.forall]
-      constructor
-      · intro h
-        rcases h with ⟨rfl, rfl⟩
-        simp
-        sorry --confident
-      · intro h
-        rcases h with ⟨h1, h2, h3⟩
-        constructor
-        · apply FullDataTree.toLeafDataTree_eq_leaf
-          · exact h2
-        · ext u d r
-          revert r
-          simp only [Option.eq_of_forall_eq]
-          have : u = () := by exact rfl
-          subst this
-          rw [h1]
-  | internal left_skeleton right_skeleton left_ih right_ih =>
-    cases leaf_data_tree with
-    | internal leftData rightData =>
-      unfold buildMerkleTree
-      simp only [simulateQ_bind, StateT.run_bind]
-      simp
-      simp [left_ih, right_ih]
-      clear left_ih right_ih
-      constructor
-      · intro h
-        rcases h with
-          ⟨left_tree, left_cache, ⟨h_left_cache, h_leftData_eq, h_left_selfConsistent⟩,
-          right_tree, right_cache, ⟨h_right_cache, h_rightData_eq, h_right_selfConsistent⟩,
-          final, h_final, h_eq⟩
-        rcases h_final with ⟨h_final_update, h_final⟩
-        -- TODO should be straightforward to rewrite everything
-        constructor
-        · intro a b r
-          clear h_leftData_eq h_rightData_eq leftData rightData
-          rw [h_final_update, Function.update_apply]
-          by_cases h_eq_a_b : (a, b) = (left_tree.getRootValue, right_tree.getRootValue)
-          · rw [h_eq_a_b]
-            simp
-            rw [<- h_eq]
-            by_cases final_eq_r : final = r
-            · simp [final_eq_r]
-            simp [final_eq_r]
-
-            sorry
-          ·
-            sorry
-
-          -- rw [h_right_cache, h_left_cache]
-
-          -- congr
-          -- rw [<- h_eq]
-          -- -- extract_goal
-          -- rw [FullDataTree.internal_toQueryCacheSet]
-          -- congr
-        · sorry
-          -- rw [h_left, h_right, ← h_eq]
-          -- rw [FullDataTree.toLeafDataTree_internal]
-      · intro h
-        rcases h with ⟨h1, h2⟩
-        -- simp [h1]
-        -- -- TODO the trees and root value can be obtained from the merkle_tree_cache
-        -- -- the query caches can be obtained by union
-        -- use merkle_tree_cache.getLeftSubtree
-        -- classical
-        -- use fun _ input => if ∃ pair : ((α × α) × α), pair.1 = input
-        --   ∧ pair ∈  then
-        --   some merkle_tree_cache.getRootValue else none
-
-        sorry
-
-
--- toVCV?
 /--
-If a final is an outcome of a run with some preexisting cache, then it is a supercache
+A functional form of the completeness theorem for Merkle trees.
 -/
-theorem subcache_of_mem_support {α β : Type} [DecidableEq α] [SelectableType α]
-    (computation : OracleComp (spec α) β)
-    (preexisting_cache resulting_cache : (spec α).QueryCache) (b : β)
-    (h_mem :
-      ((b, resulting_cache) ∈ ((simulateQ randomOracle computation).run preexisting_cache).support)
-    ) :
-    (∀ d r, preexisting_cache () d = some r → resulting_cache () d = some r) := by
-  induction computation generalizing preexisting_cache resulting_cache with
-  | pure x =>
-    intro d r h_eq
-    simp at h_eq
-    simp [StateT.run] at h_mem
-    sorry
-  | roll x r ih => sorry
-
-
-
-
--- set_option maxHeartbeats 0 in
-/--
-Characterize membership in buildMerkleTree support
-
-A merkle_tree_cache, resulting_cache pair is in the support of the
-  buildMerkleTree on leaf_data_tree simulation starting from preexisting_cache
-  iff:
-
-1. The merkle_tree_cache is the result of building a Merkle tree from the leaf_data_tree
-using the map supplied by the resulting_cache (suitably lifted to Option types)
-2. The resulting_cache is a superset of the preexisting_cache
-3. The resulting_cache does not include any entries that are not in either the
-preexisting_cache or the merkle_tree_cache.
-  1. Equivalently, If an entry is not in the preexisting_cache or the merkle_tree_cache,
-  then it is not in the resulting_cache.
-  2. Contrapositively, if an entry is in the resulting_cache, then it is either in the
-  preexisting_cache or the merkle_tree_cache.
--/
-theorem mem_buildMerkleTree_support_iff_v3 {α : Type} [DecidableEq α] [SelectableType α]
-    {s : Skeleton}
-    (leaf_data_tree : LeafDataTree α s)
-    (merkle_tree_cache : FullDataTree α s)
-    (preexisting_cache resulting_cache : (spec α).QueryCache) :
-    ((merkle_tree_cache, resulting_cache)
-      ∈ ((simulateQ randomOracle (buildMerkleTree leaf_data_tree)).run preexisting_cache).support)
-    ↔
-    (
-      (
-      -- The merkle_tree_cache is the result of building a Merkle tree from the leaf_data_tree
-      -- with the map supplied by the resulting_cache
-      merkle_tree_cache.map (Option.some) = LeafDataTree.optionComposeBuild leaf_data_tree
-        (fun a b => resulting_cache () (a, b))
-      )
-      ∧
-      -- The resulting_cache is a superset of the preexisting_cache
-      -- Note, this is needed for the rverse direction, but in the forward actuallly just a property of support membership of anything, refactor
-      (∀ d r,
-        preexisting_cache () d = some r → resulting_cache () d = some r)
-      ∧
-      -- The resulting_cache does not include any entries that are not in either the
-      -- preexisting_cache or the merkle_tree_cache
-      (∀ d r,
-        resulting_cache () d = some r →
-        (preexisting_cache () d = some r ∨ (d, r) ∈
-          merkle_tree_cache.toQueryCacheSet))
-    ) := by
-  induction s generalizing preexisting_cache resulting_cache with
+theorem functional_completeness (α : Type) {s : Skeleton}
+  (idx : SkeletonLeafIndex s)
+  (leaf_data_tree : LeafDataTree α s)
+  (hash : α → α → α) :
+  (getPutativeRoot_with_hash
+    idx
+    (leaf_data_tree.getValueAtIndex idx)
+    (generateProof
+      (buildMerkleTree_with_hash leaf_data_tree hash) idx)
+    (hash)) =
+  (buildMerkleTree_with_hash leaf_data_tree hash).getRootValue := by
+  induction s with
   | leaf =>
-    cases leaf_data_tree with
-    | leaf a =>
-      unfold buildMerkleTree
-      simp only [simulateQ_pure, StateT.run_pure, support_pure, Set.mem_singleton_iff,
-        Prod.mk.injEq, domain_def, range_def, FullDataTree.leaf_toQueryCacheSet',
-        Set.mem_empty_iff_false, or_false, Prod.forall]
-      constructor
-      · intro h
-        rcases h with ⟨rfl, rfl⟩
-        simp only [imp_self, implies_true, and_self, and_true]
-        rfl
-      · intro h
-        rcases h with ⟨h1, h2, h3⟩
-        constructor
-        · apply FullDataTree.toLeafDataTree_eq_leaf
-          simp [LeafDataTree.optionComposeBuild, LeafDataTree.map_leaf, LeafDataTree.composeBuild_leaf] at h1
-          sorry -- confident
-        · have : ∀ d r,
-              resulting_cache () d = some r ↔
-              preexisting_cache () d = some r := by
-            intro d r
-            constructor
-            · exact fun a ↦ h3 d.1 d.2 r (h2 d.1 d.2 r (h3 d.1 d.2 r a))
-            · exact fun a ↦ h2 d.1 d.2 r (h3 d.1 d.2 r (h2 d.1 d.2 r a))
-          -- simp only [Option.eq_of_forall_eq] at this
-          ext u d r
-          revert r
-          simp only [Option.eq_of_forall_eq] at this
-          have : u = () := by exact rfl
-          subst this
-          rw [this]
-          exact fun r ↦ Eq.congr_right rfl
-  | internal left_skeleton right_skeleton left_ih right_ih =>
-    cases leaf_data_tree with
-    | internal left_leaf_data right_leaf_data =>
-      unfold buildMerkleTree
-      simp only [simulateQ_bind, StateT.run_bind]
+    match leaf_data_tree with
+    | LeafDataTree.leaf a =>
       simp
-      simp [left_ih, right_ih]
-      clear left_ih right_ih
-      constructor
-      · -- Forward direction
-        intro h
-        rcases h with
-          ⟨left_tree, left_cache,
-            ⟨h_left_tree_eq_build, h_preexisting_cache_subcache_of_left_cache, h_left_cache'⟩,
-          right_tree, right_cache,
-            ⟨h_right_tree_eq_build, h_left_cache_subcache_of_right_cache, h_right_cache'⟩,
-          final, ⟨h_final_cache, h_final_cache'⟩, h_eq⟩
-        subst h_eq
-        have h_right_cache_subcache_of_resulting_cache : ∀ a b r,
-            right_cache () (a, b) = some r → resulting_cache () (a, b) = some r := by
-          sorry
-
-
-        refine ⟨?_, ?_, ?_⟩
-        · simp only [LeafDataTree.optionComposeBuild] at *
-          simp [FullDataTree.map_internal, h_left_tree_eq_build, h_right_tree_eq_build,
-            LeafDataTree.composeBuild_internal, LeafDataTree.map_internal]
-          have right_composing_cache_change :
-              (LeafDataTree.map some right_leaf_data).composeBuild
-                (Option.doubleBind fun a b ↦ right_cache () (a, b)) =
-              (LeafDataTree.map some right_leaf_data).composeBuild
-                (Option.doubleBind fun a b ↦ resulting_cache () (a, b)) := by
-            -- use right_cache_subcache_of_resulting_cache
-            sorry
-          have left_composing_cache_change :
-              (LeafDataTree.map some left_leaf_data).composeBuild
-                (Option.doubleBind fun a b ↦ left_cache () (a, b)) =
-              (LeafDataTree.map some left_leaf_data).composeBuild
-                (Option.doubleBind fun a b ↦ resulting_cache () (a, b)) := by
-            sorry
-          refine ⟨?_, ?_, ?_⟩
-          · rw [Option.some_eq_doubleBind]
-            use left_tree.getRootValue
-            use right_tree.getRootValue
-            rw [<- right_composing_cache_change, <- left_composing_cache_change]
-            rw [<-h_left_tree_eq_build, <- h_right_tree_eq_build]
-            refine ⟨?_, ?_, ?_⟩
-            · rw [FullDataTree.map_getRootValue]
-            · rw [FullDataTree.map_getRootValue]
-            · rw [h_final_cache]
-              simp
-          · exact?
-          · exact?
-
-        · intro input_left input_right output h_mem_preexisting
-          apply h_right_cache_subcache_of_resulting_cache
-          apply h_left_cache_subcache_of_right_cache
-          apply h_preexisting_cache_subcache_of_left_cache
-          exact h_mem_preexisting
-        · intro input_left input_right output h_mem_resulting
-          simp only [FullDataTree.internal_toQueryCacheSet, Set.mem_insert_iff, Prod.mk.injEq,
-            Set.mem_union]
-          -- If we sufficiently specialize the hypotheses, we can grind or aesop it out
-          -- Technically, I think we don't need to specialize the hypotheses, but aesop times out
-          -- if we don't.
-          specialize h_left_cache' input_left input_right output
-          specialize h_right_cache' input_left input_right output
-          specialize h_preexisting_cache_subcache_of_left_cache input_left input_right output
-          specialize h_left_cache_subcache_of_right_cache input_left input_right output
-          specialize h_right_cache_subcache_of_resulting_cache input_left input_right output
-          replace h_final_cache := congrFun h_final_cache (input_left, input_right)
-          simp only [Function.update_apply] at h_final_cache
-          aesop -- Sick!
-      · -- Backward direction
-        classical
-        intro h
-        have := FullDataTree.internal_eq merkle_tree_cache
-        rcases this with
-          ⟨merkle_tree_root, left_subtree, right_subtree, h_eq⟩
-        subst h_eq
-        rcases h with ⟨h1, h2, h3⟩
-        -- Construct the function for what the cache will be
-        -- after the left side of the tree is computed
-        let left_cache : (spec α).QueryCache := fun () input =>
-          if ∃ pair ∈ left_subtree.toQueryCacheSet, pair.1 = input
-          then
-            resulting_cache () input
-          else
-            preexisting_cache () input
-        use left_subtree, left_cache
-        constructor
-        · --
-          sorry
-        -- Construct the function for what the cache will be
-        -- after the right side of the tree is computed
-        let right_cache : (spec α).QueryCache := fun () input =>
-          if ∃ pair ∈ right_subtree.toQueryCacheSet, pair.1 = input
-          then
-            resulting_cache () input
-          else
-            left_cache () input
-        use right_subtree, right_cache
-        constructor
-        · sorry
-        use merkle_tree_root
-
-        sorry
-
-
-
-/--
-When generateProof runs on a cache that contains all the queries in the merkle tree,
-the putative root obtained from the resulting proof is equal to the root value of the cache.
--/
-theorem putative_root_eq_merkle_tree_cache_root_of_generate_proof {α : Type}
-    [DecidableEq α] [SelectableType α]
-    {s : Skeleton} (idx : SkeletonLeafIndex s)
-    (merkle_tree_cache : FullDataTree α s)
-    (preexisting_cache resulting_cache : (spec α).QueryCache)
-    (putative_root : α)
-    (cache_subset :
-      ∀ (a b c),
-        ((a, b), c) ∈ merkle_tree_cache.toQueryCacheSet →
-        preexisting_cache () (a, b) = some c)
-    (mem_support' :
-      (putative_root, resulting_cache) ∈
-      ((simulateQ randomOracle
-        (getPutativeRoot idx
-          ((merkle_tree_cache.toLeafDataTree).getValueAtIndex idx)
-          (generateProof merkle_tree_cache idx))).run
-        preexisting_cache).support) :
-    putative_root = merkle_tree_cache.getRootValue
-   := by
-  -- TODO refactor to avoid `QueryCache.toSet`
-  replace cache_subset :
-      merkle_tree_cache.toQueryCacheSet ⊆ QueryCache.toSet () preexisting_cache := by
-    clear mem_support'
-    simp only [Set.subset_def, QueryCache.toSet, Set.mem_setOf_eq]
-    intro x x_mem
-    apply cache_subset
-    exact x_mem
-  induction s generalizing putative_root preexisting_cache resulting_cache with
-  | leaf =>
-    cases idx with
-    | ofLeaf =>
-      simp only [generateProof_ofLeaf] at mem_support'
-      rcases mem_support' with ⟨rfl, rfl⟩
-      unfold FullDataTree.getRootValue getRootIndex
-      rw [FullDataTree.toLeafDataTree_getValueAtIndex]
+      -- unfold getPutativeRoot_with_hash
+      unfold buildMerkleTree_with_hash
       simp
+      unfold getPutativeRoot_with_hash
       rfl
-  | internal left_skeleton right_skeleton left_ih right_ih =>
-    -- Decompose the merkle tree cache into its left and right subtrees
-    have := merkle_tree_cache.internal_eq
-    rcases this with
-      ⟨merkle_tree_root, left_subtree, right_subtree, h_eq⟩
-    subst h_eq
-    cases idx with
-    | ofLeft idxLeft =>
-      simp only [generateProof_ofLeft] at mem_support'
-      unfold getPutativeRoot at mem_support'
-      simp only [simulateQ_bind, StateT.run_bind, Function.comp_apply, support_bind, Set.mem_iUnion,
-        exists_prop, Prod.exists] at mem_support'
-      simp [] at mem_support'
-      rcases mem_support' with
-        ⟨putative_root_left, cache_after_left, h_mem_left,
-        h_mem_getPutativeRoot, h_cache_after_left⟩
-      simp only [LeafDataTree.getValueAtIndex_ofLeft] at h_mem_left
-      simp at *
+  | internal s_left s_right left_ih right_ih =>
+    match leaf_data_tree with
+    | LeafDataTree.internal left right =>
+      unfold buildMerkleTree_with_hash
+      cases idx with
+      | ofLeft idxLeft =>
+        unfold getPutativeRoot_with_hash
+        simp [left_ih]
+      | ofRight idxRight =>
+        unfold getPutativeRoot_with_hash
+        simp [right_ih]
 
-      simp only [Set.insert_subset_iff, Set.union_subset_iff] at cache_subset
-      rcases cache_subset with
-        ⟨h_mem_root_compose, h_mem_left_cache_subset, h_mem_right_cache_subset⟩
-      specialize left_ih
-        idxLeft left_subtree _ cache_after_left
-        putative_root_left h_mem_left h_mem_left_cache_subset
-      have := subcache_of_mem_support (α := α) _ _ _ _
-        h_mem_left (left_subtree.getRootValue, right_subtree.getRootValue)
-      clear h_mem_left h_mem_left_cache_subset h_mem_right_cache_subset
-      subst left_ih
-      -- rcases left_ih with
-      --   ⟨putative_root_left_eq, h_preexisting_cache_subcache_of_left_cache⟩
-      -- subst putative_root_left_eq
-      simp [QueryCache.toSet] at h_mem_root_compose
-      have cache_after_left_root_compose :
-          cache_after_left () (left_subtree.getRootValue, right_subtree.getRootValue)
-          = some merkle_tree_root := by
-        aesop
-      aesop
-    | ofRight idxRight =>
-      simp only [generateProof_ofRight] at mem_support'
-      unfold getPutativeRoot at mem_support'
-      simp only [simulateQ_bind, StateT.run_bind, Function.comp_apply, support_bind, Set.mem_iUnion,
-        exists_prop, Prod.exists] at mem_support'
-      simp [] at mem_support'
-      rcases mem_support' with
-        ⟨putative_root_right, cache_after_right, h_mem_right,
-        h_mem_getPutativeRoot, h_cache_after_right⟩
-      simp only [LeafDataTree.getValueAtIndex_ofRight] at h_mem_right
-      simp at *
-      simp only [Set.insert_subset_iff, Set.union_subset_iff] at cache_subset
-      rcases cache_subset with
-        ⟨h_mem_root_compose, h_mem_left_cache_subset, h_mem_right_cache_subset⟩
-      specialize right_ih
-        idxRight right_subtree _ cache_after_right
-        putative_root_right h_mem_right h_mem_right_cache_subset
-      have := subcache_of_mem_support (α := α) _ _ _ _
-        h_mem_right (left_subtree.getRootValue, right_subtree.getRootValue)
-      clear h_mem_right h_mem_left_cache_subset h_mem_right_cache_subset
-      subst right_ih
-      -- rcases right_ih with
-      --   ⟨putative_root_right_eq, h_preexisting_cache_subcache_of_right_cache⟩
-      -- subst putative_root_right_eq
-      simp [QueryCache.toSet] at h_mem_root_compose
-      have cache_after_right_root_compose :
-          cache_after_right () (left_subtree.getRootValue, right_subtree.getRootValue)
-          = some merkle_tree_root := by
-        aesop
-      aesop
 
 theorem completeness [DecidableEq α] [SelectableType α] {s}
     (leaf_data_tree : LeafDataTree α s) (idx : BinaryTree.SkeletonLeafIndex s)
@@ -798,50 +418,15 @@ theorem completeness [DecidableEq α] [SelectableType α] {s}
       let proof := generateProof cache idx
       let _ ← verifyProof idx (leaf_data_tree.getValueAtIndex idx) (cache.getRootValue) proof
       ).simulateQ (randomOracle)).run preexisting_cache).neverFails := by
-  simp [neverFails_bind_iff]
-  constructor
-  · -- buildMerkleTree never fails
-    exact buildMerkleTree_neverFails leaf_data_tree preexisting_cache
-  · -- verifyProof never fails on the output of generateProof after buildMerkleTree
-    intros merkle_tree_cache query_cache h_mem_support
-    simp [verifyProof, neverFails_bind_iff]
-    constructor
-    · -- getPutativeRoot never fails
-      exact
-        getPutativeRoot_neverFails idx (leaf_data_tree.getValueAtIndex idx) query_cache
-          (generateProof merkle_tree_cache idx)
-    · -- guard never fails
-      intro putative_root query_cache' h_mem_support'
-      split_ifs with h
-      · -- If the putative root is equal to the root value, then we are done.
-        simp
-      -- Otherwise, we must derive a contradiction
-      simp only [StateT.run_failure, not_neverFails_failure]
-      contrapose! h
-      rw [mem_buildMerkleTree_support_iff_v3] at h_mem_support
-      rcases h_mem_support with
-        ⟨h_mem_root_compose, h_preexisting_cache_subcache_of_left_cache,
-        h_resulting_cache_subset⟩
-      have : leaf_data_tree = merkle_tree_cache.toLeafDataTree := by
-        -- follows from h_mem_root_compose
-        symm
-        exact
-          LeafDataTree.eq_full_of_map_some_eq_optionComposeBuild merkle_tree_cache leaf_data_tree
-            (fun a b ↦ query_cache () (a, b)) h_mem_root_compose
-      rw [this] at h_mem_support'
-      apply putative_root_eq_merkle_tree_cache_root_of_generate_proof
-        idx merkle_tree_cache query_cache query_cache' _ _ h_mem_support'
-      clear h_mem_support'
-
-      -- follows from h_mem_root_compose
-      intro input_left input_right output h_mem
-      have := LeafDataTree.eq_full_of_map_some_eq_optionComposeBuild'
-                merkle_tree_cache leaf_data_tree
-                (fun a b ↦ query_cache () (a, b)) h_mem_root_compose
-                input_left input_right output h_mem
-      simp at this
-      exact this
-
-end
+  revert preexisting_cache
+  rw [randomOracle_neverFails_iff_runWithOracle_neverFails]
+  intro f
+  simp only [bind_pure_comp, id_map', runWithOracle_bind, Option.bind_eq_bind]
+  rw [runWithOracle_buildMerkleTree]
+  unfold verifyProof
+  simp only [guard_eq, runWithOracle_bind]
+  simp_rw [runWithOracle_getPutativeRoot]
+  simp [apply_ite]
+  exact functional_completeness α idx leaf_data_tree fun left right ↦ f () (left, right)
 
 end InductiveMerkleTree
